How to improve the accuracy of Lattice Boltzmann calculations

Bastien Chopard

May 2008

This document is part of the LBMethod.org documentation project, and may be used under the terms of a Creative Commons Attribution-Share Alike 3.0 License. See www.lbmethod.org/legal for details.

1 A transformation of the LB dynamics

The LBGK model reads

$$f_i^{out} = f_i + \omega \left(f_i^{eq} - f_i \right) \tag{1}$$

where

$$f_i^{eq} = t_i \rho \left(1 + F_i(\mathbf{u}) \right)$$

with

$$F(\mathbf{u}) = \frac{\mathbf{u} \cdot \mathbf{v}_i}{c_s^2} + \frac{1}{2c_s^4} Q_{i\alpha\beta} u_\alpha u_\beta$$

Eq. (1) can be transformed as

$$f_i^{out} - t_i \rho_0 = f_i - t_i \rho_0 + \omega \left(f_i^{eq} - t_i \rho_0 - (f_i - t_i \rho_0) \right)$$
(2)

where ρ_0 is a constant corresponding to the average density.

Let us define

$$h_i^{out} = f_i^{out} - t_i \rho_0$$
 $h_i = f_i - t_i \rho_0$ $h_i^{eq} = f_i^{eq} - t_i \rho_0$

Then the LBGK equation becomes

$$h_i^{out} = h_i + \omega \left(h_i^{eq} - h_i \right)$$
(3)

The question is now to see whether we can simulate h_i instead of f_i . We have

$$\rho = \sum f_i = \sum h_i + \rho_0 \sum t_i = \sum h_i + \rho_0$$

because $\sum t_i = 1$. Similarly, we have

$$\mathbf{u} = \frac{\sum f_i \mathbf{v}_i}{\rho} = \frac{\sum (f_i - \rho_0 t_i) \mathbf{v}_i}{\rho}$$

because $\sum t_i \mathbf{v}_i = 0$. Then

$$\mathbf{u} = \frac{\sum h_i \mathbf{v}_i}{\rho_0 + \sum h_i}$$

In summary the density ρ and the velocity **u** can be obtained from the h_i as

$$\rho = \rho_0 + \Delta \rho \qquad \Delta \rho = \sum h_i \qquad \mathbf{u} = \frac{\sum h_i \mathbf{v}_i}{\rho_0 + \Delta \rho}$$
(4)

Note that the momentum tensor is also given by a new expression

$$\Pi_{\alpha\beta} = \sum_{i} f_{i} v_{i\alpha} v_{i\beta} = \sum_{i} h_{i} v_{i\alpha} v_{i\beta} + \sum_{i} \rho_{0} t_{i} v_{i\alpha} v_{i\beta} = \rho_{0} c_{s}^{2} \delta_{\alpha\beta} + \sum_{i} h_{i} v_{i\alpha} v_{i\beta}$$

Finally we can compute h_i^{eq}

$$h_i^{eq} = f_i^{eq} - t_i \rho_0 = t_i (\rho - \rho_0) + t_i \rho F_i(\mathbf{u})$$
(5)

Therefore

$$h_i^{eq} = t_i \Delta \rho + t_i (\rho_0 + \Delta \rho) F_i(\mathbf{u})$$
(6)

Thus the LBGK equation can be expressed in terms of the transformed distributions h_i and the value of ρ_0 .

Note that f_i is of the order $\rho_0 + Ma$ where $Ma = u/c_s$ is the Mach number which is much smaller than $\rho_0 = \mathcal{O}(1)$. This is the reason of the numerical inaccuracy of eq. (1). On the other hand, h_i is of order $\mathcal{O}(Ma)$ and so are all the terms in h^{eq} and in eq. (3).

2 Incompressible LB

In the case of the incompressible BGK models, the evaluation of h^{eq} is even simpler

$$h_i^{eq} = t_i \sum_j h_j + t_i \rho_0 F_i(\mathbf{u})$$

and \mathbf{u} becomes

$$\mathbf{u} = \frac{\sum h_i \mathbf{v}_i}{\rho_0}$$